Low_proof.v
@@ -1,0 +1,16 @@
+(* Theorems about low level protocol *)
+
+Require Import Program.
+
+Load Refinement.
+
+Theorem Low_Level_Agreement : forall params, isValidP params -> Always (compose agree ref_map) (initGS params).
+Proof.
+  unfold Always.
+  intros.
+  unfold compose.
+  eapply (HAgreement (ref_mapp params)).
+  eapply Refinement'.
+  unfold isValid.
+  auto.
+Qed.
