Temporal.v
@@ -1,0 +1,22 @@
+(* Temporal logic, monotonicity and witness theorems *)
+
+Require Import Program.
+
+Class State {A : Type} (leq : A -> A -> Prop) (nxt : A -> A) :=
+{
+  reflex : forall s, leq s s;
+  succ : forall s, leq s (nxt s);
+  transit : forall s s' s'', leq s s' -> leq s' s'' -> leq s s''
+}.
+
+Definition Next {A : Type} `{State A} (p : A -> Prop) : A -> Prop :=
+  fun s => p (nxt s).
+
+Definition Until {A : Type} `{State A} (p : A -> Prop) (q : A -> Prop) : A -> Prop :=
+  fun s => exists s'', (leq s s'' /\ q s'') /\ (forall s', leq s s' -> leq s' s'' -> p s').
+
+Definition Always {A : Type} `{State A} (p : A -> Prop) : A -> Prop :=
+  fun s => forall s', leq s s' -> p s'.
+
+Definition Eventually {A : Type} `{State A} (p : A -> Prop) : A -> Prop :=
+  fun s => exists s', leq s s' /\ p s'.
